For merge

src/Inline.v
@@ -79,7 +79,7 @@ Section Phoas.
   Fixpoint inlineDmsRep {retT} (a: Action type retT) (dms: list (DefMethT type))
            (countdown: nat): Action type retT :=
     match countdown with
-      | O => a
+      | O => inlineDms a dms
       | S cd => inlineDmsRep (inlineDms a dms) dms cd
     end.
 
@@ -280,42 +280,42 @@ Proof.
   - invertAction H0; map_simpl_G; econstructor; eauto.
 Qed.
 
-Inductive WfmActionSem: list string -> forall {retT}, Action type retT -> Prop :=
-| WfmMCallSem:
+Inductive WfmAction: list string -> forall {retT}, Action type retT -> Prop :=
+| WfmMCall:
     forall ll name sig ar {retT} cont (Hnin: ~ In name ll),
-      (forall t, WfmActionSem (name :: ll) (cont t)) ->
-      WfmActionSem ll (MCall (lretT:= retT) name sig ar cont)
-| WfmLetSem:
+      (forall t, WfmAction (name :: ll) (cont t)) ->
+      WfmAction ll (MCall (lretT:= retT) name sig ar cont)
+| WfmLet:
     forall ll {argT retT} ar cont,
-      (forall t, WfmActionSem ll (cont t)) ->
-      WfmActionSem ll (Let_ (lretT':= argT) (lretT:= retT) ar cont)
-| WfmReadRegSem:
+      (forall t, WfmAction ll (cont t)) ->
+      WfmAction ll (Let_ (lretT':= argT) (lretT:= retT) ar cont)
+| WfmReadReg:
     forall ll {retT} reg k cont,
-      (forall t, WfmActionSem ll (cont t)) ->
-      WfmActionSem ll (ReadReg (lretT:= retT) reg k cont)
-| WfmWriteRegSem:
+      (forall t, WfmAction ll (cont t)) ->
+      WfmAction ll (ReadReg (lretT:= retT) reg k cont)
+| WfmWriteReg:
     forall ll {writeT retT} reg e cont,
-      WfmActionSem ll cont ->
-      WfmActionSem ll (WriteReg (k:= writeT) (lretT:= retT) reg e cont)
-| WfmIfElseSem:
+      WfmAction ll cont ->
+      WfmAction ll (WriteReg (k:= writeT) (lretT:= retT) reg e cont)
+| WfmIfElse:
     forall ll {retT1 retT2} ce ta fa cont,
-      WfmActionSem ll (appendAction (retT1:= retT1) (retT2:= retT2) ta cont) ->
-      WfmActionSem ll (appendAction (retT1:= retT1) (retT2:= retT2) fa cont) ->
-      WfmActionSem ll (IfElse ce ta fa cont)
-| WfmAssertSem:
+      WfmAction ll (appendAction (retT1:= retT1) (retT2:= retT2) ta cont) ->
+      WfmAction ll (appendAction (retT1:= retT1) (retT2:= retT2) fa cont) ->
+      WfmAction ll (IfElse ce ta fa cont)
+| WfmAssert:
     forall ll {retT} e cont,
-      WfmActionSem ll cont ->
-      WfmActionSem ll (Assert_ (lretT:= retT) e cont)
-| WfmReturnSem:
-    forall ll {retT} (e: Expr type retT), WfmActionSem ll (Return e).
+      WfmAction ll cont ->
+      WfmAction ll (Assert_ (lretT:= retT) e cont)
+| WfmReturn:
+    forall ll {retT} (e: Expr type retT), WfmAction ll (Return e).
 
-Hint Constructors WfmActionSem.
+Hint Constructors WfmAction.
 
-Lemma WfmActionSem_init_sub:
+Lemma WfmAction_init_sub:
   forall {retK} (a: Action type retK) ll1
-         (Hwfm: WfmActionSem ll1 a) ll2
+         (Hwfm: WfmAction ll1 a) ll2
          (Hin: forall k, In k ll2 -> In k ll1),
-    WfmActionSem ll2 a.
+    WfmAction ll2 a.
 Proof.
   induction 1; intros; simpl; intuition.
 
@@ -324,11 +324,11 @@ Proof.
   intros; inv H1; intuition.
 Qed.
 
-Lemma WfmActionSem_append_1':
+Lemma WfmAction_append_1':
   forall {retT2} a3 ll,
-    WfmActionSem ll a3 ->
+    WfmAction ll a3 ->
     forall {retT1} (a1: Action type retT1) (a2: type retT1 -> Action type retT2),
-      a3 = appendAction a1 a2 -> WfmActionSem ll a1.
+      a3 = appendAction a1 a2 -> WfmAction ll a1.
 Proof.
   induction 1; intros.
 
@@ -343,30 +343,30 @@ Proof.
     econstructor; eauto.
   - destruct a1; simpl in *; try discriminate; inv H1; destruct_existT.
     constructor.
-    + eapply IHWfmActionSem1; eauto; apply appendAction_assoc.
-    + eapply IHWfmActionSem2; eauto; apply appendAction_assoc.
+    + eapply IHWfmAction1; eauto; apply appendAction_assoc.
+    + eapply IHWfmAction2; eauto; apply appendAction_assoc.
   - destruct a1; simpl in *; try discriminate; inv H0; destruct_existT.
     econstructor; eauto.
   - destruct a1; simpl in *; try discriminate.
 Qed.
 
-Lemma WfmActionSem_append_1:
+Lemma WfmAction_append_1:
   forall {retT1 retT2} (a1: Action type retT1) (a2: type retT1 -> Action type retT2) ll,
-    WfmActionSem ll (appendAction a1 a2) ->
-    WfmActionSem ll a1.
-Proof. intros; eapply WfmActionSem_append_1'; eauto. Qed.
+    WfmAction ll (appendAction a1 a2) ->
+    WfmAction ll a1.
+Proof. intros; eapply WfmAction_append_1'; eauto. Qed.
 
-Lemma WfmActionSem_append_2':
+Lemma WfmAction_append_2':
   forall {retT2} a3 ll,
-    WfmActionSem ll a3 ->
+    WfmAction ll a3 ->
     forall {retT1} (a1: Action type retT1) (a2: type retT1 -> Action type retT2),
       a3 = appendAction a1 a2 ->
-      forall t, WfmActionSem ll (a2 t).
+      forall t, WfmAction ll (a2 t).
 Proof.
   induction 1; intros.
 
   - destruct a1; simpl in *; try discriminate; inv H1; destruct_existT.
-    apply WfmActionSem_init_sub with (ll1:= meth :: ll); [|intros; right; assumption].
+    apply WfmAction_init_sub with (ll1:= meth :: ll); [|intros; right; assumption].
     eapply H0; eauto.
   - destruct a1; simpl in *; try discriminate; inv H1; destruct_existT.
     + eapply H0; eauto.
@@ -374,12 +374,12 @@ Proof.
   - destruct a1; simpl in *; try discriminate; inv H1; destruct_existT.
     eapply H0; eauto.
   - destruct a1; simpl in *; try discriminate; inv H0; destruct_existT.
-    eapply IHWfmActionSem; eauto.
+    eapply IHWfmAction; eauto.
   - destruct a1; simpl in *; try discriminate; inv H1; destruct_existT.
-    eapply IHWfmActionSem1; eauto.
+    eapply IHWfmAction1; eauto.
     apply appendAction_assoc.
   - destruct a1; simpl in *; try discriminate; inv H0; destruct_existT.
-    eapply IHWfmActionSem; eauto.
+    eapply IHWfmAction; eauto.
   - destruct a1; simpl in *; try discriminate.
 
     Grab Existential Variables.
@@ -388,16 +388,16 @@ Proof.
     { exact (evalConstT (getDefaultConst _)). }    
 Qed.
 
-Lemma WfmActionSem_append_2:
+Lemma WfmAction_append_2:
   forall {retT1 retT2} (a1: Action type retT1) (a2: type retT1 -> Action type retT2) ll,
-    WfmActionSem ll (appendAction a1 a2) ->
-    forall t, WfmActionSem ll (a2 t).
-Proof. intros; eapply WfmActionSem_append_2'; eauto. Qed.
+    WfmAction ll (appendAction a1 a2) ->
+    forall t, WfmAction ll (a2 t).
+Proof. intros; eapply WfmAction_append_2'; eauto. Qed.
 
-Lemma WfmActionSem_cmMap:
+Lemma WfmAction_cmMap:
   forall {retK} olds (a: Action type retK) news calls retV ll
          (Hsem: SemAction olds a news calls retV)
-         (Hwfm: WfmActionSem ll a)
+         (Hwfm: WfmAction ll a)
          lb (Hin: In lb ll),
     find lb calls = None.
 Proof.
@@ -405,7 +405,7 @@ Proof.
 
   - rewrite find_add_2.
     { apply IHHsem; eauto.
-      specialize (H2 mret); eapply WfmActionSem_init_sub; eauto.
+      specialize (H2 mret); eapply WfmAction_init_sub; eauto.
       intros; right; assumption.
     }
     { unfold string_eq; destruct (string_dec _ _); [subst; elim Hnin; assumption|intuition]. }
@@ -414,30 +414,30 @@ Proof.
   - eapply IHHsem; eauto.
   - assert (find lb calls1 = None).
     { eapply IHHsem1; eauto.
-      eapply WfmActionSem_append_1; eauto.
+      eapply WfmAction_append_1; eauto.
     }
     assert (find lb calls2 = None).
     { eapply IHHsem2; eauto.
-      eapply WfmActionSem_append_2; eauto.
+      eapply WfmAction_append_2; eauto.
     }
     repeat autounfold with MapDefs in *.
     rewrite H, H0; reflexivity.
   - assert (find lb calls1 = None).
     { eapply IHHsem1; eauto.
-      eapply WfmActionSem_append_1; eauto.
+      eapply WfmAction_append_1; eauto.
     }
     assert (find lb calls2 = None).
     { eapply IHHsem2; eauto.
-      eapply WfmActionSem_append_2; eauto.
+      eapply WfmAction_append_2; eauto.
     }
     repeat autounfold with MapDefs in *.
     rewrite H, H0; reflexivity.
   - eapply IHHsem; eauto.
 Qed.
 
-Lemma WfmActionSem_append_3':
+Lemma WfmAction_append_3':
   forall {retT2} a3 ll,
-    WfmActionSem ll a3 ->
+    WfmAction ll a3 ->
     forall {retT1} (a1: Action type retT1) (a2: type retT1 -> Action type retT2),
       a3 = appendAction a1 a2 ->
       forall olds1 olds2 news1 news2 calls1 calls2 retV1 retV2,
@@ -452,78 +452,104 @@ Proof.
     specialize (H0 _ _ _ _ eq_refl _ _ _ _ _ _ _ _ H1 H3 lb).
     destruct H0; [|right; assumption].
     destruct (string_dec lb meth); [subst; right|left].
-    + pose proof (WfmActionSem_append_2 _ _ H retV1).
-      eapply WfmActionSem_cmMap; eauto.
+    + pose proof (WfmAction_append_2 _ _ H retV1).
+      eapply WfmAction_cmMap; eauto.
     + rewrite find_add_2; [assumption|unfold string_eq; destruct (string_dec _ _); intuition].
 
   - inv H1; destruct_existT; invertAction H2; eapply H0; eauto.
   - inv H1; destruct_existT; invertAction H2; left; reflexivity.
   - inv H1; destruct_existT; invertAction H2; eapply H0; eauto.
-  - inv H0; destruct_existT; invertAction H1; eapply IHWfmActionSem; eauto.
+  - inv H0; destruct_existT; invertAction H1; eapply IHWfmAction; eauto.
   - inv H1; destruct_existT.
     invertAction H2.
     destruct (evalExpr e); dest; subst.
-    + specialize (@IHWfmActionSem1 _ (appendAction a1_1 a) a2 (appendAction_assoc _ _ _)).
-      eapply IHWfmActionSem1; eauto.
+    + specialize (@IHWfmAction1 _ (appendAction a1_1 a) a2 (appendAction_assoc _ _ _)).
+      eapply IHWfmAction1; eauto.
       instantiate (1:= union x x1); instantiate (1:= olds1).
       eapply appendAction_SemAction_2; eauto.
       intuition.
-    + specialize (@IHWfmActionSem2 _ (appendAction a1_2 a) a2 (appendAction_assoc _ _ _)).
-      eapply IHWfmActionSem2; eauto.
+    + specialize (@IHWfmAction2 _ (appendAction a1_2 a) a2 (appendAction_assoc _ _ _)).
+      eapply IHWfmAction2; eauto.
       instantiate (1:= union x x1); instantiate (1:= olds1).
       eapply appendAction_SemAction_2; eauto.
       intuition.
     
-  - inv H0; destruct_existT; invertAction H1; eapply IHWfmActionSem; eauto.
+  - inv H0; destruct_existT; invertAction H1; eapply IHWfmAction; eauto.
 Qed.
 
-Lemma WfmActionSem_append_3:
+Lemma WfmAction_append_3:
   forall {retT1 retT2} (a1: Action type retT1) (a2: type retT1 -> Action type retT2) ll,
-    WfmActionSem ll (appendAction a1 a2) ->
+    WfmAction ll (appendAction a1 a2) ->
     forall olds1 olds2 news1 news2 calls1 calls2 retV1 retV2,
       SemAction olds1 a1 news1 calls1 retV1 ->
       SemAction olds2 (a2 retV1) news2 calls2 retV2 ->
       forall lb, find lb calls1 = None \/ find lb calls2 = None.
-Proof. intros; eapply WfmActionSem_append_3'; eauto. Qed.
+Proof. intros; eapply WfmAction_append_3'; eauto. Qed.
 
-Lemma WfmActionSem_init:
+Lemma WfmAction_init:
   forall {retK} (a: Action type retK) ll
-         (Hwfm: WfmActionSem ll a),
-    WfmActionSem nil a.
-Proof. intros; eapply WfmActionSem_init_sub; eauto; intros; inv H. Qed.
+         (Hwfm: WfmAction ll a),
+    WfmAction nil a.
+Proof. intros; eapply WfmAction_init_sub; eauto; intros; inv H. Qed.
 
-Lemma WfmActionSem_MCall:
-  forall {retK} olds a news calls (retV: type retK) dmn
+Lemma WfmAction_MCall:
+  forall {retK} olds a news calls (retV: type retK) dms
          (Hsem: SemAction olds a news calls retV)
-         (Hwfm: WfmActionSem [dmn] a),
-    complement calls [dmn] = calls.
+         (Hwfm: WfmAction dms a),
+    complement calls dms = calls.
 Proof.
   induction 1; intros; inv Hwfm; destruct_existT.
 
   - rewrite complement_add_2 by assumption; f_equal.
     apply IHHsem.
     specialize (H2 mret).
-    apply (WfmActionSem_init_sub H2 [dmn]).
-    intros; inv H; intuition.
+    apply (WfmAction_init_sub H2 dms).
+    intros; right; assumption.
   - eapply IHHsem; eauto.
   - eapply IHHsem; eauto.
   - eapply IHHsem; eauto.
   - rewrite complement_union; f_equal.
     + eapply IHHsem1; eauto.
-      eapply WfmActionSem_append_1; eauto.
+      eapply WfmAction_append_1; eauto.
     + eapply IHHsem2; eauto.
-      eapply WfmActionSem_append_2; eauto.
+      eapply WfmAction_append_2; eauto.
   - rewrite complement_union; f_equal.
     + eapply IHHsem1; eauto.
-      eapply WfmActionSem_append_1; eauto.
+      eapply WfmAction_append_1; eauto.
     + eapply IHHsem2; eauto.
-      eapply WfmActionSem_append_2; eauto.
+      eapply WfmAction_append_2; eauto.
   - eapply IHHsem; eauto.
   - map_simpl_G; reflexivity.
 Qed.
 
-Lemma inlineDm_not_called:
-  forall {retK} olds (a: Action type retK) news calls retV dm
+(* TODO: weird definition *)
+Inductive WfmDms: list (DefMethT type) -> Prop :=
+| WfmDmsNil: WfmDms nil
+| WfmDmsCons: forall (dm: DefMethT type) dms,
+                (forall arg, WfmAction (map (@attrName _) dms) (objVal (attrType dm) arg)) ->
+                ~ In (attrName dm) (map (@attrName _) dms) ->
+                WfmDms dms -> WfmDms (dm :: dms).
+
+Inductive SoundInlineDms: forall {retT}, Action type retT -> list (DefMethT type) -> Prop :=
+| SoundInlineDmsNil: forall {retT} (a: Action type retT), WfmAction nil a -> SoundInlineDms a nil
+| SoundInlineDmsCons:
+    forall {retT} (a: Action type retT) (dm: DefMethT type) dms,
+      WfmAction nil (inlineDm a dm) ->
+      SoundInlineDms (inlineDm a dm) dms ->
+      SoundInlineDms a (dm :: dms).
+
+Inductive SoundInlineDmsRep:
+  forall {retT}, Action type retT -> list (DefMethT type) -> nat -> Prop :=
+| SoundInlineDmsO: forall {retT} (a: Action type retT) dms,
+                     SoundInlineDms a dms -> SoundInlineDmsRep a dms O
+| SoundInlineDmsS:
+    forall {retT} (a: Action type retT) dms n,
+      SoundInlineDms (inlineDms a dms) dms ->
+      SoundInlineDmsRep (inlineDms a dms) dms n ->
+      SoundInlineDmsRep a dms (S n).
+
+Lemma inlineDm_SemAction_not_called:
+  forall {retK} (a: Action type retK) olds news calls retV dm
          (Hsem: SemAction olds a news calls retV)
          (Hcol: find (attrName dm) calls = None),
     SemAction olds (inlineDm a dm) news calls retV.
@@ -587,11 +613,12 @@ Section Preliminaries.
     forall olds1 olds2 retK2 a2
            dm rules news1 news2 dmMap1 cmMap1 cmMap2
            (retV2: type retK2),
-      Disj olds1 olds2 -> Disj news1 news2 -> Disj cmMap1 cmMap2 ->
-      
-      WfmActionSem nil a2 ->
+      (* Disj olds1 olds2 -> *)
+      (Disj olds1 olds2 \/ FnMap.Sub olds1 olds2) ->
+      Disj news1 news2 -> Disj cmMap1 cmMap2 ->
+      WfmAction nil a2 ->
+
       SemAction olds2 a2 news2 cmMap2 retV2 ->
-      
       find (attrName dm) cmMap2 = find (attrName dm) dmMap1 -> (* labels match *)
       DomainOf dmMap1 ((attrName dm) :: nil) -> (* dm is actually called *)
       
@@ -623,13 +650,26 @@ Section Preliminaries.
         simpl in *; rewrite <-Eqdep.EqdepTheory.eq_rect_eq; clear e0.
 
         econstructor; eauto.
-        apply appendAction_SemAction_1 with (retV1:= x0); auto.
-        map_simpl_G.
+        destruct H3.
 
-        inv H2; destruct_existT.
-        specialize (H8 x0).
-        pose proof (WfmActionSem_MCall H5 H8); rewrite H.
-        assumption.
+        * apply appendAction_SemAction_1 with (retV1:= x0); auto.
+          map_simpl_G.
+          
+          inv H2; destruct_existT.
+          specialize (H8 x0).
+          pose proof (WfmAction_MCall H5 H8). rewrite H2.
+          assumption.
+
+        * apply appendAction_SemAction_2 with (olds1:= olds1) (retV1:= x0); auto.
+          { apply Sub_union. }
+          { map_simpl_G.
+
+            inv H2; destruct_existT.
+            specialize (H8 x0).
+            pose proof (WfmAction_MCall H5 H8). rewrite H2.
+            rewrite Sub_merge by assumption.
+            assumption.
+          }
 
       + rewrite find_add_2 in H4
           by (unfold string_eq; destruct (string_dec _ _); [elim n; assumption|reflexivity]).
@@ -665,7 +705,7 @@ Section Preliminaries.
         * apply H; auto.
           { inv H2; destruct_existT.
             specialize (H10 x1).
-            eapply WfmActionSem_init; eauto.
+            eapply WfmAction_init; eauto.
           }
           { eapply Disj_add_2; eauto. }
 
@@ -673,7 +713,10 @@ Section Preliminaries.
       simpl; econstructor; eauto.
     - invertAction H5; inv H2; destruct_existT.
       simpl; econstructor; eauto.
-      apply Disj_find_union; eauto.
+
+      destruct H3.
+      + apply Disj_find_union; eauto.
+      + rewrite Sub_merge; assumption.
     - invertAction H3; inv H2; destruct_existT.
       simpl; econstructor; eauto.
       + instantiate (1:= union news1 x1).
@@ -703,7 +746,7 @@ Section Preliminaries.
 
           { auto. }
           { eapply IHa2_1. 
-            { eapply WfmActionSem_append_1; eauto. }
+            { eapply WfmAction_append_1; eauto. }
             { instantiate (1:= x2); eapply Disj_union_1; eauto. }
             { auto. }
             { instantiate (1:= x1); eapply Disj_union_1; eauto. }
@@ -711,18 +754,21 @@ Section Preliminaries.
             { exact H2. }
           }
           { instantiate (1:= x4); instantiate (1:= x3).
-            apply inlineDm_not_called.
-            { eapply action_olds_ext; eauto.
-              rewrite Disj_union_unionR by assumption.
-              apply Sub_unionR.
+            apply inlineDm_SemAction_not_called.
+            { destruct H3.
+              { eapply action_olds_ext; eauto.
+                rewrite Disj_union_unionR by assumption.
+                apply Sub_unionR.
+              }
+              { rewrite Sub_merge; assumption. }
             }
-            { pose proof (WfmActionSem_append_3 _ H11 H2 H5 dmn).
+            { pose proof (WfmAction_append_3 _ H11 H2 H5 dmn).
               destruct H6; [|assumption].
               rewrite H6 in Heqdmv1; discriminate.
             }
           }
           { apply union_assoc. }
-          { pose proof (WfmActionSem_append_3 _ H11 H2 H5 dmn).
+          { pose proof (WfmAction_append_3 _ H11 H2 H5 dmn).
             destruct H6; [rewrite H6 in Heqdmv1; discriminate|].
             assert (complement x4 [dmn] = x4).
             { clear -H6.
@@ -738,15 +784,18 @@ Section Preliminaries.
 
           { auto. }
           { instantiate (1:= x5); instantiate (1:= x2); instantiate (1:= x1).
-            apply inlineDm_not_called.
-            { eapply action_olds_ext; eauto.
-              rewrite Disj_union_unionR by assumption.
-              apply Sub_unionR.
+            apply inlineDm_SemAction_not_called.
+            { destruct H3.
+              { eapply action_olds_ext; eauto.
+                rewrite Disj_union_unionR by assumption.
+                apply Sub_unionR.
+              }
+              { rewrite Sub_merge; assumption. }
             }
             { auto. }
           }
           { apply H.
-            { eapply WfmActionSem_append_2; eauto. }
+            { eapply WfmAction_append_2; eauto. }
             { instantiate (1:= x4); eapply Disj_union_2; eauto. }
             { repeat autounfold with MapDefs in *.
               rewrite <-Heqdmv1 in H4; assumption.
@@ -785,7 +834,7 @@ Section Preliminaries.
 
           { auto. }
           { eapply IHa2_2. 
-            { eapply WfmActionSem_append_1; eauto. }
+            { eapply WfmAction_append_1; eauto. }
             { instantiate (1:= x2); eapply Disj_union_1; eauto. }
             { auto. }
             { instantiate (1:= x1); eapply Disj_union_1; eauto. }
@@ -793,18 +842,21 @@ Section Preliminaries.
             { exact H2. }
           }
           { instantiate (1:= x4); instantiate (1:= x3).
-            apply inlineDm_not_called.
-            { eapply action_olds_ext; eauto.
-              rewrite Disj_union_unionR by assumption.
-              apply Sub_unionR.
+            apply inlineDm_SemAction_not_called.
+            { destruct H3.
+              { eapply action_olds_ext; eauto.
+                rewrite Disj_union_unionR by assumption.
+                apply Sub_unionR.
+              }
+              { rewrite Sub_merge; assumption. }
             }
-            { pose proof (WfmActionSem_append_3 _ H15 H2 H5 dmn).
+            { pose proof (WfmAction_append_3 _ H15 H2 H5 dmn).
               destruct H6; [|assumption].
               rewrite H6 in Heqdmv1; discriminate.
             }
           }
           { apply union_assoc. }
-          { pose proof (WfmActionSem_append_3 _ H15 H2 H5 dmn).
+          { pose proof (WfmAction_append_3 _ H15 H2 H5 dmn).
             destruct H6; [rewrite H6 in Heqdmv1; discriminate|].
             assert (complement x4 [dmn] = x4).
             { clear -H6.
@@ -820,15 +872,18 @@ Section Preliminaries.
 
           { auto. }
           { instantiate (1:= x5); instantiate (1:= x2); instantiate (1:= x1).
-            apply inlineDm_not_called.
-            { eapply action_olds_ext; eauto.
-              rewrite Disj_union_unionR by assumption.
-              apply Sub_unionR.
+            apply inlineDm_SemAction_not_called.
+            { destruct H3.
+              { eapply action_olds_ext; eauto.
+                rewrite Disj_union_unionR by assumption.
+                apply Sub_unionR.
+              }
+              { rewrite Sub_merge; assumption. }
             }
             { auto. }
           }
           { apply H.
-            { eapply WfmActionSem_append_2; eauto. }
+            { eapply WfmAction_append_2; eauto. }
             { instantiate (1:= x4); eapply Disj_union_2; eauto. }
             { repeat autounfold with MapDefs in *.
               rewrite <-Heqdmv1 in H4; assumption.
@@ -866,6 +921,11 @@ Section Preliminaries.
   Lemma inlineDms_prop:
     forall dms olds1 olds2 retK2 a2 rules news1 news2 dmMap1 cmMap1 cmMap2
            (retV2: type retK2),
+      (Disj olds1 olds2 \/ FnMap.Sub olds1 olds2) ->
+      Disj news1 news2 -> Disj cmMap1 cmMap2 ->
+      WfmAction nil a2 ->
+      WfmDms dms -> SoundInlineDms a2 dms ->
+
       SemAction olds2 a2 news2 cmMap2 retV2 ->
       dmMap1 = restrict cmMap2 (map (@attrName _) dms) ->
       SemMod rules olds1 None news1 dms dmMap1 cmMap1 ->
@@ -873,8 +933,203 @@ Section Preliminaries.
                 (union news1 news2) (union cmMap1 (complement cmMap2 (map (@attrName _) dms)))
                 retV2.
   Proof.
-    admit.
+    induction dms; intros.
+
+    - inv H7; map_simpl_G; simpl.
+      destruct H.
+      + eapply action_olds_ext; eauto.
+        rewrite Disj_union_unionR; auto.
+        apply Sub_unionR.
+      + rewrite Sub_merge; assumption.
+
+    - inv H7.
+      
+      + assert (complement cmMap2 (map (@attrName _) (a :: dms)) =
+                complement (complement cmMap2 [attrName a]) (map (@attrName _) dms)); dest.
+        { clear.
+          apply Equal_eq; repeat autounfold with MapDefs; intros.
+          destruct (in_dec _ k (map (@attrName _) (a :: dms))).
+          { inv i.
+            { destruct (in_dec _ (attrName a) (map (@attrName _) dms)); [reflexivity|].
+              destruct (in_dec _ _ _); [reflexivity|].
+              elim n0; left; reflexivity.
+            }
+            { destruct (in_dec _ k (map (@attrName _) dms)); [reflexivity|elim n; assumption]. }
+          }
+          { destruct (in_dec _ k (map (@attrName _) dms)); [elim n; right; assumption|].
+            destruct (in_dec _ k [attrName a]); [|reflexivity].
+            inv i; [|inv H].
+            elim n; left; reflexivity.
+          }
+        }
+        rewrite H6; clear H6; simpl.
+        
+        rewrite <-union_idempotent with (m:= olds1).
+        rewrite union_comm with (m1:= news).
+        rewrite union_comm with (m1:= calls).
+        repeat rewrite <-union_assoc.
+
+        assert (calls = complement calls (map (@attrName _) dms)).
+        { inv H3; specialize (H8 argV).
+          pose proof (WfmAction_MCall HAction H8); auto.
+        }
+        rewrite H6; clear H6.
+        rewrite <-complement_union.
+
+        eapply IHdms.
+        { right; apply Sub_union. }
+        { apply Disj_union.
+          { apply Disj_comm; auto. }
+          { apply Disj_comm; apply Disj_comm in H0; apply Disj_union_2 in H0; auto. }
+        }
+        { apply Disj_union.
+          { apply Disj_comm; auto. }
+          { apply Disj_complement.
+            apply Disj_comm; apply Disj_comm in H1; apply Disj_union_2 in H1; auto.
+          }
+        }
+        { inv H4; destruct_existT. assumption. }
+        { inv H3; auto. }
+        { inv H4; destruct_existT; auto. }
+        { eapply inlineDm_prop.
+          { assumption. }
+          { apply Disj_comm in H0; apply Disj_comm.
+            eapply Disj_union_1; eauto.
+          }
+          { apply Disj_comm in H1; apply Disj_comm.
+            eapply Disj_union_1; eauto.
+          }
+          { assumption. }
+          { assumption. }
+          { instantiate (1:= add a {| objType := objType (attrType a);
+                                      objVal := (argV, retV) |} empty).
+            map_compute_G.
+            apply Equal_val with (k:= a) in HDefs; map_compute HDefs.
+            assumption.
+          }
+          { clear.
+            unfold DomainOf; intros; unfold InMap;
+            repeat autounfold with MapDefs; split; intros.
+            { unfold string_eq in H; destruct (string_dec _ _); intuition idtac.
+              subst; left; reflexivity.
+            }
+            { inv H; [|inv H0]; map_compute_G; discriminate. }
+          }
+          { instantiate (1:= rules).
+            eapply SemAddMeth; eauto.
+            { apply Disj_empty_2. }
+            { apply Disj_empty_2. }
+          }
+        }
+        { instantiate (1:= dm2).
+          inv H3; specialize (H8 argV).
+          pose proof (WfmAction_MCall HAction H8).
+          apply complement_restrict_nil in H3.
+          rewrite restrict_union; rewrite H3.
+          rewrite union_empty_1.
+          pose proof (SemMod_dmMap_InDomain HSemMod).
+
+          (* Low-level map property - couldn't find proper lemmas *)
+          clear -HDefs H6 H9.
+          apply Equal_eq; repeat autounfold with MapDefs in *; intro k.
+          apply @Equal_val with (k := k) in HDefs.
+          specialize (H6 k).
+          destruct (in_dec _ k (map (@attrName _) dms)).
+          { destruct (in_dec _ k (map (@attrName _) (a :: dms)));
+            [clear i0|elim n; right; assumption].
+            destruct (in_dec _ k [attrName a]).
+            { inv i0; [|inv H]; elim H9; assumption. }
+            { unfold string_eq in HDefs.
+              destruct (string_dec a k); [|auto].
+              subst; elim n; left; reflexivity.
+            }
+          }
+          { destruct (in_dec _ _ _).
+            { inv i; [|elim n; assumption].
+              map_compute HDefs.
+              destruct (dm2 a); [|reflexivity].
+              elim n; apply H6; discriminate.
+            }
+            { unfold string_eq in HDefs.
+              destruct (string_dec _ _); [|auto].
+              subst; elim n0; left; reflexivity.
+            }
+          }
+        }
+        { eassumption. }
+        { assumption. }
+        { assumption. }
+
+      + inv H3.
+        assert (find a cmMap2 = None).
+        { pose proof (SemMod_dmMap_InDomain HSemMod); clear -H3 H9.
+          repeat autounfold with MapDefs in *.
+          specialize (H3 a).
+          destruct (in_dec _ _ _); [clear i|elim n; left; reflexivity].
+          destruct (cmMap2 a); [|reflexivity].
+          elim H9; apply H3; discriminate.
+        }
+
+        assert (restrict cmMap2 (map (@attrName _) (a :: dms)) =
+                restrict cmMap2 (map (@attrName _) dms) /\
+                complement cmMap2 (map (@attrName _) (a :: dms)) =
+                complement cmMap2 (map (@attrName _) dms)); dest.
+        { clear -H3 H9; split.
+          { apply Equal_eq; repeat autounfold with MapDefs in *; intros k.
+            destruct (in_dec _ k (map (@attrName _) (a :: dms))).
+            { destruct (in_dec _ k (map (@attrName _) dms)); [reflexivity|].
+              inv i; [assumption|elim n; assumption].
+            }
+            { destruct (in_dec _ _ _); [elim n; right; assumption|reflexivity]. }
+          }
+          { apply Equal_eq; repeat autounfold with MapDefs in *; intros k.
+            destruct (in_dec _ _ (map (@attrName _) (a :: dms))).
+            { destruct (in_dec _ _ _); [reflexivity|].
+              inv i; [auto|elim n; assumption].
+            }
+            { destruct (in_dec _ _ _); [|reflexivity].
+              elim n; right; assumption.
+            }
+          }
+        }
+        rewrite H6 in HSemMod; rewrite H7; clear H6 H7.
+
+        simpl; eapply IHdms.
+        { assumption. }
+        { assumption. }
+        { assumption. }
+        { inv H4; destruct_existT; auto. }
+        { inv H3; auto. }
+        { inv H4; destruct_existT; auto. }
+        { apply inlineDm_SemAction_not_called; auto. }
+        { reflexivity. }
+        { eassumption. }
+        
   Qed.
+
+  (* problem: SemMod varies for each countdown step *)
+  Lemma inlineDmsRep_prop:
+    forall dms countdown olds1 olds2 retK2 a2 rules news1 news2 dmMap1 cmMap1 cmMap2
+           (retV2: type retK2),
+      (Disj olds1 olds2 \/ FnMap.Sub olds1 olds2) ->
+      Disj news1 news2 -> Disj cmMap1 cmMap2 ->
+      WfmAction nil a2 ->
+      WfmDms dms -> SoundInlineDmsRep a2 dms countdown ->
+
+      SemAction olds2 a2 news2 cmMap2 retV2 ->
+      dmMap1 = restrict cmMap2 (map (@attrName _) dms) ->
+      SemMod rules olds1 None news1 dms dmMap1 cmMap1 ->
+      SemAction (union olds1 olds2) (inlineDmsRep a2 dms countdown)
+                (union news1 news2) (union cmMap1 (complement cmMap2 (map (@attrName _) dms)))
+                retV2.
+  Proof.
+    induction countdown; intros;
+    [simpl; inv H4; destruct_existT; eapply inlineDms_prop; eauto|].
+
+    simpl; eapply IHcountdown; try assumption.
+
+    - 
+      
 
   (* TODO: extend *)
 
